Tests/Ignore.lean
@@ -1,5 +1,7 @@
 import Qed
 
+set_option autoImplicit false
+
 open Qed.Ignore
 
 -- fnmatch: exact match
